examples/sha3/proofs/Sha3/Equivalence.lean
@@ -11,6 +11,12 @@ namespace sha3
 open Std.Do Aeneas
 set_option mvcgen.warning false
 
+set_option trace.Hax.hax_mvcgen_at true
+
+attribute [spec] KeccakState.Insts.CoreOpsIndexIndexPairUsizeUsizeT.index
+attribute [spec] get_ij
+attribute [spec] U64.Insts.Sha3KeccakItem1.xor_constant _veorq_n_u64 KeccakState.set set_ij
+
 theorem iota_spec
   (st : KeccakState U64.Insts.Sha3KeccakItem1) (i : Std.Usize)
   (h : (_requires_iota st i).holds):
@@ -18,3 +24,32 @@ theorem iota_spec
     iota st i
     ⦃ ⇓ r => ⌜ (_ensures_iota st i r).holds ⌝ ⦄ := by
   hax_mvcgen [iota, KeccakState.iota, _requires_iota]
+  mspec
+  mspec
+  sorry
+  hax_mvcgen
+  mspec
+  sorry
+  hax_mvcgen
+  mspec
+  sorry
+  hax_mvcgen
+  mspec
+  mspec
+  sorry
+  hax_mvcgen
+  mspec
+  mspec
+  hax_mvcgen
+  mspec
+  mspec
+  sorry
+  hax_mvcgen
+  mspec
+  sorry
+  hax_mvcgen
+  mspec
+  sorry
+  hax_mvcgen
+  mspec
+  sorry
